wip

extraction/lib/DynamicShim.ml
@@ -8,54 +8,26 @@ module type DYNAMIC_ARRANGEMENT = sig
   type name
   type state
   type msg
-  type res = state * (name * msg) list
+  type timeout
+  type res = state * (name * msg) list * timeout list * timeout list
   val addr_of_name : name -> (string * int)
   val name_of_addr : (string * int) -> name
-  val is_request : msg -> bool
-  val closes_request : msg -> msg -> bool
   val init : name -> name list -> res
   val handleNet : name -> name -> msg -> state -> res
-  val handleTick : name -> state -> res
-  val handleTimeout : name -> name -> state -> res
-  val setTick : name -> state -> float
-  val query_timeout : float
+  val handleTimeout : name -> state -> timeout -> res
+  val setTimeout : timeout -> float
+  val default_timeout : float
   val debug : bool
   val debugRecv : state -> (name * msg) -> unit
   val debugSend : state -> (name * msg) -> unit
-  val debugTick : state -> unit
-  val debugTimeout : state -> (name * msg) -> unit
+  val debugTimeout : state -> timeout -> unit
 end
 module Shim (A: DYNAMIC_ARRANGEMENT) = struct
   (* assoc list of start times mapping to (name, msg) pairs *)
 
-  type requests = (float * A.name * A.msg) list
-  let empty_requests = []
-
-  let rec timed_out_requests timeout ts : (A.name * A.msg) list =
-    let now = Unix.gettimeofday () in
-    match ts with
-    | (t, dst, msg) :: rest ->
-       if now -. t > timeout
-       then (dst, msg) :: timed_out_requests timeout rest
-       else timed_out_requests timeout rest
-    | [] -> []
-
-  let rec record_request rs (dst, msg) : requests =
-    if A.is_request msg
-    then (Unix.gettimeofday (), dst, msg) :: rs
-    else rs
-
-  let remove_requests rs dst : requests =
-    List.filter (fun (_, d, _) -> d != dst) rs
-
-  let close_requests rs src res : requests =
-    let not_closed (_, nm, req) = not (A.closes_request req res) in
-    List.filter not_closed rs
-
   type env =
     {
       usock : file_descr;
-      mutable open_requests : requests;
       mutable last_tick : float
     }
 
@@ -64,7 +36,6 @@ module Shim (A: DYNAMIC_ARRANGEMENT) = struct
     let port = snd (A.addr_of_name nm) in
     let env =
       { usock = socket PF_INET SOCK_DGRAM 0;
-        open_requests = empty_requests;
         last_tick = Unix.gettimeofday ()
       }
     in
@@ -87,13 +58,18 @@ module Shim (A: DYNAMIC_ARRANGEMENT) = struct
 
   let respond_one env s p =
     (if A.debug then A.debugSend s p);
-    env.open_requests <- record_request env.open_requests p;
     send env p
 
-  let respond env (s, ps) =
-    List.iter (respond_one env s) ps; s
+  let add_time t =
+    (A.setTimeout t, t)
 
-  let recv_step env nm s =
+  let respond env ts (s, ps, newts, clearedts) =
+    let ts' = (List.filter (fun (_, t) -> not (List.mem t clearedts)) ts)
+              @ (List.map add_time newts) in
+    List.iter (respond_one env s) ps;
+    s, ts'
+
+  let recv_step env nm s ts =
     let len = 4096 in
     let buf = String.make len '\x00' in
     let (_, from) = recvfrom env.usock buf 0 len [] in
@@ -102,47 +78,49 @@ module Shim (A: DYNAMIC_ARRANGEMENT) = struct
      | ADDR_UNIX _ -> failwith "UNEXPECTED MESSAGE FROM UNIX ADDR"
      | ADDR_INET (addr,port) -> A.name_of_addr (string_of_inet_addr addr, port)) in
     let m = unpack_msg buf in
-    let s' = respond env (A.handleNet src nm m s) in
+    let (s', ts') = respond env ts (A.handleNet src nm m s) in
     (if A.debug then A.debugRecv s' (src, m));
-    env.open_requests <- close_requests env.open_requests src m;
-    s'
-
-  let tick_step env nm s =
-    (if A.debug then A.debugTick s);
-    env.last_tick <- Unix.gettimeofday ();
-    let x = A.handleTick nm s in
-    respond env x
-
-  let do_timeout env nm (s, sends) (dst, msg) =
-    let (s', sends') = A.handleTimeout nm dst s in
-    env.open_requests <- remove_requests env.open_requests dst;
-    A.debugTimeout s (dst, msg);
-    (s', sends @ sends')
-
-  let timeout_step env nm s =
-    let timeouts = timed_out_requests A.query_timeout env.open_requests in
-    let res = List.fold_left (do_timeout env nm) (s, []) timeouts in
-    respond env res
-
-  let maybe_tick env nm s =
-    if (Unix.gettimeofday ()) -. env.last_tick > A.setTick nm s
-    then tick_step env nm s
-    else s
+    s', ts'
 
   let rec my_select rs ws es t =
     try select rs ws es t
     with Unix_error (err, fn, arg) ->
       my_select rs ws es t
 
-  let rec eloop env nm s =
-    let (fds, _, _) = my_select [env.usock] [] [] (A.setTick nm s) in
-    let s' = if List.mem env.usock fds
-             then (try (recv_step env nm s) with
-                   | _ -> s)
-             else s in
-    let s'' = timeout_step env nm s' in
-    let s''' = maybe_tick env nm s'' in
-    eloop env nm s'''
+  let rec uniqappend l =
+    function
+    | [] -> l
+    | (h :: rest) -> if List.mem h l
+                     then uniqappend l rest
+                     else uniqappend (l @ [h]) rest
+
+  let do_timeout env nm (s, sends, newts, clearedts) (deadline, t) =
+    if not (List.mem t clearedts)
+    then let (s', sends', newts', clearedts') = (A.handleTimeout nm s t) in
+         (s', sends @ sends', newts @ newts', uniqappend clearedts clearedts')
+    else (s, sends, newts, clearedts)
+    
+  let timeout_step env nm s ts =
+    let now = Unix.gettimeofday () in
+    let live = List.filter (fun (d, _) -> now > d) ts in
+    let (s, sends, newts, clearedts) = List.fold_left (do_timeout env nm) (s, [], [], []) live in
+    respond env ts (s, sends, newts, uniqappend clearedts (List.map snd live))
+
+  let min_of_list default l =
+    List.fold_left (fun acc x -> min acc x) default l
+
+  let free_time ts =
+    let now = Unix.gettimeofday () in
+    max A.default_timeout ((min_of_list now (List.map fst ts)) -. now)
+
+  let rec eloop env nm (s, ts) =
+    let (fds, _, _) = my_select [env.usock] [] [] (free_time ts) in
+    let (s', ts') = if List.mem env.usock fds
+             then (try (recv_step env nm s ts) with
+                   | _ -> (s, ts))
+             else (s, ts) in
+    let (s'', ts'') = timeout_step env nm s' ts in
+    eloop env nm (s'', ts'')
 
   let default v o =
     match o with
@@ -153,5 +131,5 @@ module Shim (A: DYNAMIC_ARRANGEMENT) = struct
     print_endline "running setup";
     let env = setup nm in
     print_endline "starting";
-    eloop env nm (respond env (A.init nm knowns));
+    eloop env nm (respond env [] (A.init nm knowns));
 end
