systems/Chord.v
@@ -35,7 +35,34 @@ Section Chord.
   | Ping : payload
   | Pong : payload.
 
+  Inductive timeout :=
+  | Tick : timeout
+  | Request : addr -> payload -> timeout.
+
+  Inductive query :=
+  (* needs a pointer to the notifier *)
+  | Rectify : pointer -> query
+  | Stabilize : query
+  (* needs a new successor *)
+  | Stabilize2 : pointer -> query
+  (* needs a known node *)
+  | Join : pointer -> query
+  (* needs to know new successor *)
+  | Join2 : pointer -> query.
+
+  Record data := Data { ptr : pointer ;
+                        pred : option pointer ;
+                        succ_list : list pointer ;
+                        known : pointer ;
+                        joined : bool ;
+                        rectify_with : option pointer ;
+                        cur_request : option (pointer * query * payload) ;
+                        query_sent : bool }.
+
+  Definition res := (data * list (addr * payload) * list timeout * list timeout)%type.
+
   Definition client_payload msg := exists (p : pointer), msg = GetBestPredecessor p.
+
   Inductive request_payload : payload -> Prop :=
   | req_GetBestPredecessor : forall m p, m = GetBestPredecessor p -> request_payload m
   | req_GetSuccList : request_payload GetSuccList
@@ -75,31 +102,11 @@ Section Chord.
   Definition can_be_client (a : addr) := True.
   Definition can_be_node (a : addr) := True.
 
-  Inductive query :=
-  (* needs a pointer to the notifier *)
-  | Rectify : pointer -> query
-  | Stabilize : query
-  (* needs a new successor *)
-  | Stabilize2 : pointer -> query
-  (* needs a known node *)
-  | Join : pointer -> query
-  (* needs to know new successor *)
-  | Join2 : pointer -> query.
-
-  Record data := Data { ptr : pointer ;
-                        pred : option pointer ;
-                        succ_list : list pointer ;
-                        known : pointer ;
-                        joined : bool ;
-                        rectify_with : option pointer ;
-                        cur_request : option (pointer * query) ;
-                        query_sent : bool }.
-
   Definition update_pred (st : data) (p : pointer) := Data (ptr st) (Some p) (succ_list st) (known st) (joined st) (rectify_with st) (cur_request st) (query_sent st).
 
   Definition update_succ_list (st : data) (succs : list pointer) := Data (ptr st) (pred st) succs (known st) (joined st) (rectify_with st) (cur_request st) (query_sent st).
 
-  Definition update_query (st : data) (dst : pointer) (q : query) := Data (ptr st) (pred st) (succ_list st) (known st) (joined st) (rectify_with st) (Some (dst, q)) (query_sent st).
+  Definition update_query (st : data) (dst : pointer) (q : query) (m : payload) := Data (ptr st) (pred st) (succ_list st) (known st) (joined st) (rectify_with st) (Some (dst, q, m)) (query_sent st).
 
   Definition update_for_join (st : data) (succs : list pointer) := Data (ptr st) None succs (known st) true (rectify_with st) (cur_request st) (query_sent st).
 
@@ -117,42 +124,50 @@ Section Chord.
                             end
       | Stabilize => match head (succ_list st) with
                        | Some succ => Some (succ, GetPredAndSuccs)
-                       | None => None (* should not happen in a good network *)
+                       | None => None (* impossible under protocol assumptions but possible irl *)
                      end
       | Stabilize2 new_succ => Some (new_succ, GetSuccList)
       | Join known => Some (known, GetBestPredecessor (make_pointer h))
       | Join2 new_succ => Some (new_succ, GetSuccList)
     end.
 
-  Definition start_query (h : addr) (st : data) (k : query) : data * list (addr * payload) :=
+  Definition timeouts_in (st : data) : list timeout :=
+    match cur_request st with
+      | Some (dst, q, m) => [Request (addr_of dst) m]
+      | None => []
+    end. 
+
+  Definition start_query (h : addr) (st : data) (k : query) : res :=
+    let cst := timeouts_in st in
     match make_request h st k with
-      | Some (dst, msg) => (update_query st dst k, [(addr_of dst, msg)])
-      | None => (st, []) (* should not happen *)
+      | Some (dst, msg) => (update_query st dst k msg, [(addr_of dst, msg)], [Request (addr_of dst) msg], cst)
+      | None => (st, [], [], []) (* only happens if succ_list = [], which is contra protocol assumptions *)
     end.
 
   (* something to prove: try_rectify is not invoked unless cur_request st is None *)
-  Definition try_rectify (h : addr) (outs : list (addr * payload)) (st : data) : data * list (addr * payload) :=
+  Definition try_rectify (h : addr) (outs : list (addr * payload)) (st : data) : res :=
     if joined st
     then match rectify_with st with
            | Some new => match pred st with
                            | Some _ => let st' := clear_rectify_with st in
-                                       let (st'', outs') := start_query h st' (Rectify new) in
-                                       (st'', outs ++ outs')
+                                       let '(st'', outs', nts, cts) := start_query h st' (Rectify new) in
+                                       (st'', outs ++ outs', nts, cts)
                            | None => let st' := clear_rectify_with (update_pred st new) in
-                                     (st', outs)
+                                     (st', outs, [], [])
                          end
-           | None => (st, outs)
+           | None => (st, outs, [], [])
          end
-    else (st, outs).
+    else (st, outs, [], []).
 
   Definition request_in (msgs : list (addr * payload)) :=
     existsb is_request (map snd msgs).
 
-  Definition end_query (h : addr) (res : data * list (addr * payload)) : data * list (addr * payload) :=
-    let (st, outs) := res in
+  Definition end_query (h : addr) (r : res) : res :=
+    let '(st, outs, nts, cts) := r in
     let st' := Data (ptr st) (pred st) (succ_list st) (known st) (joined st) (rectify_with st) None false in
+    let clearreq := timeouts_in st in
     if request_in outs
-    then (st', outs)
+    then (st', outs, nts, cts ++ clearreq)
     else try_rectify h outs st'.
 
   Definition ptrs_to_addrs : list (pointer * payload) -> list (addr * payload) :=
@@ -186,77 +201,77 @@ Section Chord.
          | None => h
        end.
 
-  Definition handle_rectify (h : addr) (st : data) (my_pred : pointer) (q : query) (notifier : pointer) : data * list (addr * payload) :=
+  Definition handle_rectify (h : addr) (st : data) (my_pred : pointer) (q : query) (notifier : pointer) : res :=
     if between_bool (id_of my_pred) (id_of notifier) (id_of (ptr st))
-    then (update_pred st notifier, [])
-    else (st, []).
+    then (update_pred st notifier, [], [], [])
+    else (st, [], [], []).
 
-  Definition handle_stabilize (h : addr) (src : pointer) (st : data) (q : query) (new_succ : pointer) (succs : list pointer) : data * list (addr * payload) :=
+  Definition handle_stabilize (h : addr) (src : pointer) (st : data) (q : query) (new_succ : pointer) (succs : list pointer) : res :=
     let new_st := update_succ_list st (make_succs src succs) in
     if between_bool (id_of (ptr st)) (id_of new_succ) (id_of src)
     then start_query h new_st (Stabilize2 new_succ)
-    else end_query h (new_st, [(addr_of src, Notify)]).
+    else end_query h (new_st, [(addr_of src, Notify)], [], []).
 
-  Definition handle_query (src : addr) (h : addr) (st : data) (qdst : pointer) (q : query) (msg : payload) : data * list (addr * payload) :=
+  Definition handle_query (src : addr) (h : addr) (st : data) (qdst : pointer) (q : query) (msg : payload) : res :=
     match q with
       | Rectify notifier =>
         match msg with
           | Pong => match (pred st) with
                       | Some p => end_query h (handle_rectify h st p q notifier)
-                      | None => end_query h (update_pred st notifier, [])
+                      | None => end_query h (update_pred st notifier, [], [], [])
                     end
-          | _ => (st, [])
+          | _ => (st, [], [], [])
         end
       | Stabilize =>
         match msg with
           | GotPredAndSuccs new_succ succs =>
             match new_succ with
               | Some ns => (handle_stabilize h (make_pointer src) st q ns succs)
-              | None => end_query h (st, [])
+              | None => end_query h (st, [], [], [])
             end
-          | _ => (st, [])
+          | _ => (st, [], [], [])
         end
       | Stabilize2 new_succ =>
         match msg with
           | GotSuccList succs => end_query h (update_succ_list st (make_succs new_succ succs),
-                                              [(addr_of new_succ, Notify)])
-          | _ => (st, [])
+                                              [(addr_of new_succ, Notify)], [], [])
+          | _ => (st, [], [], [])
         end
       | Join known =>
         match msg with
           | GotBestPredecessor p => let a := addr_of p in
                                     if addr_eq_dec a src
-                                    then (st, [(src, GetSuccList)])
-                                    else (st, [(a, GetBestPredecessor (make_pointer h))])
+                                    then (st, [(src, GetSuccList)], [], [])
+                                    else (st, [(a, GetBestPredecessor (make_pointer h))], [], [])
           | GotSuccList l =>
             match l with
-              | [] => end_query h (st, []) (* this is bad *)
+              | [] => end_query h (st, [], [], []) (* this is bad *)
               | (new_succ :: _) => start_query (addr_of new_succ) st (Join2 new_succ)
             end
-          | _ => (st, [])
+          | _ => (st, [], [], [])
         end
       | Join2 new_succ =>
         match msg with
           | GotSuccList l => let succs := make_succs new_succ l in
-                             end_query h (update_for_join st succs, [])
-          | _ => (st, [])
+                             end_query h (update_for_join st succs, [], [], [])
+          | _ => (st, [], [], [])
         end
     end.
 
-  Definition recv_handler (src : addr) (dst : addr) (msg : payload) (st : data) : data * list (addr * payload) :=
+  Definition recv_handler (src : addr) (dst : addr) (msg : payload) (st : data) : res :=
     match msg with
-      | Ping => (st, [(src, Pong)])
-      | GetSuccList => (st, [(src, GotSuccList (succ_list st))])
-      | GetPredAndSuccs => (st, [(src, GotPredAndSuccs (pred st) (succ_list st))])
-      | GetBestPredecessor p => (st, [(src, GotBestPredecessor (best_predecessor (ptr st) (succ_list st) (id_of p)))])
-      | Notify => (set_rectify_with st (make_pointer src), [])
+      | Ping => (st, [(src, Pong)], [], [])
+      | GetSuccList => (st, [(src, GotSuccList (succ_list st))], [], [])
+      | GetPredAndSuccs => (st, [(src, GotPredAndSuccs (pred st) (succ_list st))], [], [])
+      | GetBestPredecessor p => (st, [(src, GotBestPredecessor (best_predecessor (ptr st) (succ_list st) (id_of p)))], [], [])
+      | Notify => (set_rectify_with st (make_pointer src), [], [], [])
       | _ => match cur_request st with
-               | Some (query_dst, q) => handle_query src dst st query_dst q msg
-               | None => (st, [])
+               | Some (query_dst, q, _) => handle_query src dst st query_dst q msg
+               | None => (st, [], [], [])
              end
     end.
 
-  Definition start_handler (h : addr) (knowns : list addr) : data * list (addr * payload) :=
+  Definition start_handler (h : addr) (knowns : list addr) : res :=
     match knowns with
       | k :: [] =>
         let known := make_pointer k in
@@ -266,42 +281,42 @@ Section Chord.
         let p := make_pointer k in
         let succs := chop_succs (map make_pointer nowns) in
         let st := Data (make_pointer h) (Some p) succs p true None None false in
-        (st, [])
+        (st, [], [], [])
       (* garbage data, shouldn't happen *)
-      | [] => (Data (make_pointer h) None [] (make_pointer h) false None None false, [])
+      | [] => (Data (make_pointer h) None [] (make_pointer h) false None None false, [], [], [])
     end.
 
-  Definition tick_handler (h : addr) (st : data) : data * list (addr * payload) :=
+  Definition tick_handler (h : addr) (st : data) : res :=
     match cur_request st with
-      | Some _ => (st, [])
+      | Some _ => (st, [], [], [])
       | None => if joined st
                 then start_query h st Stabilize
-                else (st, []) (*start_query h st (Join (known st))*)
+                else (st, [], [], []) (*start_query h st (Join (known st))*)
     end.
 
-  Definition handle_query_timeout (h : addr) (st : data) (dead : pointer) (q : query) : data * list (addr * payload) :=
+  Definition handle_query_timeout (h : addr) (st : data) (dead : pointer) (q : query) : res :=
     match q with
-      | Rectify notifier => end_query h (update_pred st notifier, [])
+      | Rectify notifier => end_query h (update_pred st notifier, [], [], [])
       | Stabilize =>
         match succ_list st with
           | _ :: rest => start_query h (update_succ_list st rest) Stabilize
-          | [] => end_query h (st, []) (* should not happen in a good network *)
+          | [] => end_query h (st, [], [], []) (* should not happen in a good network *)
         end
       | Stabilize2 new_succ =>
         match succ_list st with
-          | next :: _ => end_query h (st, [(addr_of next, Notify)])
-          | [] => end_query h (st, []) (* again, this shouldn't happen *)
+          | next :: _ => end_query h (st, [(addr_of next, Notify)], [], [])
+          | [] => end_query h (st, [], [], []) (* again, this shouldn't happen *)
         end
-      | Join known => end_query h (st, [])
-      | Join2 new_succ => end_query h (st, [])
+      | Join known => end_query h (st, [], [], [])
+      | Join2 new_succ => end_query h (st, [], [], [])
     end.
 
-  Definition timeout_handler (src : addr) (dst : addr) (st : data) : data * list (addr * payload) :=
+  Definition timeout_handler (src : addr) (dst : addr) (st : data) : res :=
     match cur_request st with
-      | Some (ptr, q) => if addr_eq_dec (addr_of ptr) dst
+      | Some (ptr, q, _) => if addr_eq_dec (addr_of ptr) dst
                          then handle_query_timeout src st ptr q
-                         else (st, []) (* shouldn't happen *)
-      | None => (st, []) (* shouldn't happen *)
+                         else (st, [], [], []) (* shouldn't happen *)
+      | None => (st, [], [], []) (* shouldn't happen *)
     end.
 
   Lemma is_request_same_as_request_payload : forall msg : payload,
@@ -321,9 +336,9 @@ Section Chord.
     - induction msg; intuition; inversion H; inversion H0.
   Qed.
 
-  Lemma requests_are_always_responded_to : forall src dst msg st sends,
+  Lemma requests_are_always_responded_to : forall src dst msg st sends nts cts,
       request_payload msg ->
-      (st, sends) = recv_handler src dst msg st ->
+      (st, sends, nts, cts) = recv_handler src dst msg st ->
       exists res, In (src, res) sends.
   Proof.
     intuition.
