extraction/chord/coq/ExtractChord.v
@@ -10,16 +10,20 @@ Definition SUCC_LIST_LEN := 5.
 Definition hash (a : addr) : id :=
   a mod 256.
 
-Definition handleNet : addr -> addr -> payload -> data -> data * list (addr * payload) :=
+Definition handleNet : addr -> addr -> payload -> data -> res :=
   recv_handler SUCC_LIST_LEN hash.
 
-Definition init : addr -> list addr -> data * list (addr * payload) :=
+Definition init : addr -> list addr -> res :=
   start_handler SUCC_LIST_LEN hash.
 
-Definition handleTick : addr -> data -> data * list (addr * payload) :=
+Definition handleTick : addr -> data -> res :=
   tick_handler hash.
 
-Definition handleTimeout : addr -> addr -> data -> data * list (addr * payload) :=
+Definition handleTimeout : addr -> addr -> data -> res :=
   timeout_handler hash.
 
+Definition test (a b c : nat) : nat * nat * nat :=
+  (a, b, c).
+
+Extraction "Test.ml" test.
 Extraction "ExtractedChord.ml" init handleNet handleTick handleTimeout is_request closes_request.
